fix bug in prepare phase

ver3_less_complex/Replica.dfy
@@ -49,10 +49,10 @@ module M_Replica {
     requires ReplicaInit(r, r.id)
     ensures ValidReplicaState(r)
     {
-        // assert Inv_Blockchain_Inner_Consistency(r.bc);
-        // assert r.commitQC.CertNone?;
-        // assert r.prepareQC.CertNone?;
-        // assert r.bc == [M_SpecTypes.Genesis_Block];
+        assert r.commitQC.CertNone?;
+        assert r.prepareQC.CertNone?;
+        assert r.bc == [M_SpecTypes.Genesis_Block];
+        assert r.msgSent == {};
     }
 
     lemma LemmaReplicaNextSubIsValid(r : ReplicaState, r' : ReplicaState, outMsg : set<Msg>)
@@ -82,7 +82,8 @@ module M_Replica {
             }
             else
             {
-                // UponNextView, UponTimeOut are proved automatically by Dafny
+                LemmaValidationHoldsInNewViewPhase(r, r', outMsg);
+                // UponTimeOut are proved automatically by Dafny
             }
         }
     }
@@ -111,7 +112,15 @@ module M_Replica {
             assert ReplicaNextSubStep(s[|s|-2], s[|s|-1], o[|s|-2]);
             LemmaReplicaNextSubIsValid(s[|s|-2], s[|s|-1], o[|s|-2]);
         }
-        
+    }
+
+    lemma LemmaReplicaNextSubStable(r : ReplicaState, r' : ReplicaState, outMsg : set<Msg>)
+    requires ValidReplicaState(r)
+    requires ReplicaNextSubStep(r, r', outMsg)
+    ensures r'.msgReceived == r.msgReceived
+    ensures r'.msgSent == r.msgSent + outMsg
+    {
+
     }
 
     lemma LemmaMsgRelationInReplicaNext(
@@ -121,8 +130,8 @@ module M_Replica {
         outMsg : set<Msg>)
     requires ValidReplicaState(r)
     requires ReplicaNext(r, inMsg, r', outMsg)
-    ensures r.msgReceived + inMsg <= r'.msgReceived
-    ensures r'.msgReceived - r.msgReceived <= outMsg
+    ensures r'.msgReceived == r.msgReceived + inMsg
+    // ensures r'.msgReceived - r.msgReceived <= outMsg
     ensures r'.msgSent == r.msgSent + outMsg
     {
         var allMsgReceived := r.msgReceived + inMsg;
@@ -139,18 +148,29 @@ module M_Replica {
                     && ReplicaNextSubStep(s[i], s[i+1], o[i])
                 )
                 && outMsg == setUnionOnSeq(o);
+        // assert s[0].msgReceived == r.msgReceived + inMsg;
+        // var msgSeq := mapSeq(s, getMsgReceive);
+        // LemmaSetEqualityTransitiveInSeq(msgSeq);
+        // assert s[0].msgReceived == s[|s|-1].msgReceived;
+        // var msg : set<Msg> := getMsgReceive(s[0]);
+        var msgRecSeq := mapSeq(s, getMsgReceiveReplica);
+        var msgSentSeq := mapSeq(s, getMsgSentReplica);
+        assert s[|s|-1].msgReceived == s[0].msgReceived by {
+            forall i | 0 <= i < |s|-1 
+            ensures msgRecSeq[i] == msgRecSeq[i+1] {
+                LemmaReplicaNextSubStable(s[i], s[i+1], o[i]);
+            }
+            LemmaSetEqualityTransitiveInSeq(msgRecSeq);
+        }
 
-        var msgSeq := mapSeq(s, getMsgReceive);
-        LemmaSubsetTransitiveInSeq(msgSeq);
-        // assert s[0].msgReceived <= s[|s|-1].msgReceived by {
-        //     forall i | 0 <= i < |s|-1 
-        //     ensures msgSeq[i] <= msgSeq[i+1] {
-        //         assert msgSeq[i] == getMsgReceive(s[i]);
-        //         assert s[i].msgReceived <= s[i+1].msgReceived;
-        //         assert msgSeq[i] <= msgSeq[i+1];
-        //     }
-        //     LemmaSubsetTransitiveInSeq(msgSeq);
-        // }
+        assert s[|s|-1].msgSent == s[0].msgSent + outMsg by {
+            forall i | 0 < i < |s|
+            ensures msgSentSeq[i] == msgSentSeq[i-1] + o[i-1] {
+                LemmaReplicaNextSubStable(s[i-1], s[i], o[i-1]);
+            }
+            LemmaSeqCumulative(msgSentSeq, o);
+        }
+
     }
 
     lemma LemmaSubsetTransitive(a : set, b : set, c : set)
@@ -241,23 +261,9 @@ module M_Replica {
               || UponCommit(r, r', outMsg)
               || UponDecide(r, r', outMsg)
               ) 
-    // requires UponTimeOut(r, r', outMsg)     
-    // requires UponPrepare(r, r', outMsg)      
-    // requires UponPreCommit(r, r', outMsg)    
-    // requires UponCommit(r, r', outMsg)       
-    // requires UponDecide(r, r', outMsg)
     ensures ValidReplicaState(r')
     {
-        // var leader := leader(r.viewNum);
-        // if (leader == r.id){
-        //     calc {
-        //         r'.msgReceived;
-        //         >=
-        //         r.msgReceived;
-        //     }
-        // }
-        // else {  // OBSERVE
-        // }
+        LemmaReplicaNextSubIsValid(r, r', outMsg);
     }
 
     lemma LemmaValidationHoldsInPreparePhase(r : ReplicaState, r' : ReplicaState, outMsg : set<Msg>)
@@ -289,6 +295,10 @@ module M_Replica {
     ensures r'.msgReceived == r.msgReceived
     {
         assert r'.viewNum == r.viewNum;
+        assert r'.prepareQC == r.prepareQC;
+        assert r'.bc == r.bc;
+        assert r'.id == r.id;
+        assert r'.msgReceived == r.msgReceived;
     }
 
     lemma LemmaValidationHoldsInPreCommitPhase(r : ReplicaState, r' : ReplicaState, outMsg : set<Msg>)
@@ -459,59 +469,107 @@ module M_Replica {
     }
 
 
+    lemma LemmaValidationHoldsInNewViewPhase(r : ReplicaState, r' : ReplicaState, outMsg : set<Msg>)
+    requires ValidReplicaState(r)
+    requires UponNextView(r, r', outMsg)
+    ensures ValidReplicaState(r')
+    {
+    }
+
+    // predicate UponPrepare(r : ReplicaState, r' : ReplicaState, outMsg: set<Msg>)
+    // requires ValidReplicaState(r)
+    // {
+    //     var leader := leader(r.viewNum);
+    //     if leader == r.id // Leader
+    //     then
+    //         // assume r.viewNum > 0;
+    //         var matchMsgs := getMatchMsg(r.msgReceived, MT_NewView, r.viewNum-1);
+    //         var highQC := getHighQC(matchMsgs);
+    //         var proposal := getNewBlock(highQC.block);
+    //         var proposeMsg := Msg(MT_Prepare, r.viewNum, proposal, highQC, SigNone);
+    //         var matchMsgs2 := getMatchProposalMsg(r.msgReceived + {proposeMsg}, r.viewNum);
+    //         && (forall m | m in matchMsgs2 ::
+    //                 // var sig := Signature(r.id, m.mType, m.viewNum, m.block);
+    //                 // var vote := Msg(MT_Prepare, r.viewNum, m.block, CertNone, sig);
+    //                 var vote := buildVoteMsg(MT_Prepare, m.block, CertNone, r.viewNum, r.id);
+    //                 // assert vote.mType.MT_Prepare?;
+    //                 // assert vote == vote2;
+    //                 if  && m.block.Block?
+    //                     && m.justify.Cert? 
+    //                     && extension(m.block, m.justify.block) 
+    //                     && r.commitQC.Cert?
+    //                     && safeNode(m.block, m.justify, r.commitQC)
+    //                 then
+    //                     // && outMsg == {vote, proposeMsg}
+    //                     && outMsg == outMsg + {vote, proposeMsg}
+    //                 else
+    //                     // && outMsg == {proposeMsg}
+    //                     && outMsg == outMsg + {proposeMsg}
+    //             )
+    //         && r' == r.(msgReceived := r.msgReceived + {proposeMsg},
+    //                     msgSent := r.msgSent + outMsg)
+    //     else
+    //         // var matchMsgs := getMatchMsg(r.msgReceived, MT_Prepare, r.viewNum);
+    //         var matchMsgs := getMatchProposalMsg(r.msgReceived, r.viewNum);
+    //         (&& (forall m | m in matchMsgs ::
+    //                 // var sig := Signature(r.id, m.mType, m.viewNum, m.block);
+    //                 // var vote2 := Msg(MT_Prepare, r.viewNum, m.block, CertNone, sig);
+    //                 var vote := buildVoteMsg(MT_Prepare, m.block, CertNone, r.viewNum, r.id);
+    //                 // assert vote == vote2;
+    //                 if  && m.block.Block?
+    //                     && m.justify.Cert? 
+    //                     && extension(m.block, m.justify.block) 
+    //                     && r.commitQC.Cert?
+    //                     && safeNode(m.block, m.justify, r.commitQC)
+    //                 then
+    //                     && outMsg == {vote}
+    //                 else
+    //                     && outMsg == {}
+    //             )
+    //         && r' == r.(msgSent := r.msgSent + outMsg)
+    //         )
+    // }
+
+    // Refactor for outMsg (28/11/2025)
     predicate UponPrepare(r : ReplicaState, r' : ReplicaState, outMsg: set<Msg>)
     requires ValidReplicaState(r)
-    // ensures ValidReplicaState(r')
     {
         var leader := leader(r.viewNum);
         if leader == r.id // Leader
         then
             // assume r.viewNum > 0;
+            var matchProposals := getMatchProposalMsg(r.msgReceived, r.viewNum);
+            var votes := getVotesForSafeProposals(matchProposals, r.commitQC, r.id);
+            var filteredVotes := proposalVoteFilter(votes);
             var matchMsgs := getMatchMsg(r.msgReceived, MT_NewView, r.viewNum-1);
-            var highQC := getHighQC(matchMsgs);
-            var proposal := getNewBlock(highQC.block);
-            var proposeMsg := Msg(MT_Prepare, r.viewNum, proposal, highQC, SigNone);
-
-            // var matchMsgs2 := getMatchMsg(r.msgReceived + {proposeMsg}, MT_Prepare, r.viewNum);
-            var matchMsgs2 := getMatchProposalMsg(r.msgReceived + {proposeMsg}, r.viewNum);
-            && (forall m | m in matchMsgs2 ::
-                    // var sig := Signature(r.id, m.mType, m.viewNum, m.block);
-                    // var vote := Msg(MT_Prepare, r.viewNum, m.block, CertNone, sig);
-                    var vote := buildVoteMsg(MT_Prepare, m.block, CertNone, r.viewNum, r.id);
-                    // assert vote == vote2;
-                    if  && m.block.Block?
-                        && m.justify.Cert? 
-                        && extension(m.block, m.justify.block) 
-                        && r.commitQC.Cert?
-                        && safeNode(m.block, m.justify, r.commitQC)
-                    then
-                        && outMsg == {vote, proposeMsg}
-                    else
-                        && outMsg == {proposeMsg}
-                )
-            && r' == r.(msgReceived := r.msgReceived + {proposeMsg},
-                        msgSent := r.msgSent + outMsg)
+            if |matchMsgs| > 0
+            then
+                var highQC := getHighQC(matchMsgs);
+                var proposal := getNewBlock(highQC.block);
+                var proposeMsg := Msg(MT_Prepare, r.viewNum, proposal, highQC, SigNone);
+                // var matchProposals := getMatchProposalMsg(r.msgReceived + {proposeMsg}, r.viewNum);
+                && outMsg == filteredVotes + {proposeMsg}
+                && r' == r.(msgSent := r.msgSent + filteredVotes + {proposeMsg})
+            else
+                && outMsg == filteredVotes
+                && r' == r.(msgSent := r.msgSent + filteredVotes)
         else
-            // var matchMsgs := getMatchMsg(r.msgReceived, MT_Prepare, r.viewNum);
-            var matchMsgs := getMatchProposalMsg(r.msgReceived, r.viewNum);
-            (&& (forall m | m in matchMsgs ::
-                    // var sig := Signature(r.id, m.mType, m.viewNum, m.block);
-                    // var vote2 := Msg(MT_Prepare, r.viewNum, m.block, CertNone, sig);
-                    var vote := buildVoteMsg(MT_Prepare, m.block, CertNone, r.viewNum, r.id);
-                    // assert vote == vote2;
-                    if  && m.block.Block?
-                        && m.justify.Cert? 
-                        && extension(m.block, m.justify.block) 
-                        && r.commitQC.Cert?
-                        && safeNode(m.block, m.justify, r.commitQC)
-                    then
-                        && outMsg == {vote}
-                    else
-                        && outMsg == {}
-                )
+            var matchProposals := getMatchProposalMsg(r.msgReceived, r.viewNum);
+            // NoOuterClient();
+            var votes := getVotesForSafeProposals(matchProposals, r.commitQC, r.id);
+            var filteredVotes := proposalVoteFilter(votes);
+            && outMsg == filteredVotes
             && r' == r.(msgSent := r.msgSent + outMsg)
-            )
     }
+
+    lemma setEqualityTest<T>(s1 : set<T>, s2 : set<T>, p : T -> bool)
+    requires s1 == s2
+    ensures (forall e | e in s1 
+                    :: p(e))
+            ==>
+            (forall e | e in s2
+                    :: p(e))
+    {}
 
     ghost predicate UponPreCommit(r : ReplicaState, r' : ReplicaState, outMsg : set<Msg>)
     requires ValidReplicaState(r)
@@ -531,7 +589,7 @@ module M_Replica {
                 var vote := buildVoteMsg(MT_PreCommit, m_qc.block, CertNone, r.viewNum, r.id);
                 // assert vote == vote2;
                 // assert vote.mType == MT_PreCommit;
-                var matchMsgs := getMatchMsg(r.msgReceived, MT_Prepare, r.viewNum);
+                var matchMsgs := getMatchVoteMsg(r.msgReceived, MT_Prepare, r.viewNum);
                 // What if these message contain different voted blocks?
                 // Split thess message by responding block, and get the group with the most elements.
                 var splitSets := splitMsgByBlocks(matchMsgs);
@@ -542,54 +600,36 @@ module M_Replica {
                     var m :| m in maxSet;
                     var sgns := ExtractSignatrues(maxSet);
                     var prepareQC := Cert(MT_Prepare, m.viewNum, m.block, sgns);
+                    // assert ValidQC(prepareQC);
                     var precommitMsg := Msg(MT_PreCommit, r.viewNum, EmptyBlock, prepareQC, SigNone);
                     assert ValidQC(m_qc);
-                    assert m_qc == prepareQC;
                     && outMsg == {vote, precommitMsg}
-                    && r' == r.(msgReceived := r.msgReceived + {precommitMsg},
-                                msgSent := r.msgSent + {vote, precommitMsg},
-                                prepareQC := m_qc)
+                    && r' == r.(prepareQC := m_qc,
+                                msgSent := r.msgSent + {vote, precommitMsg})
                 else
                     assert ValidQC(m_qc);
                     && outMsg == {vote}
                     && r' == r.(prepareQC := m_qc,
                                 msgSent := r.msgSent + {vote})
             else    // Only doing leader's work
-                var matchMsgs := getMatchMsg(r.msgReceived, MT_Prepare, r.viewNum);
+                var matchMsgs := getMatchVoteMsg(r.msgReceived, MT_Prepare, r.viewNum);
                 var splitSets := splitMsgByBlocks(matchMsgs);
                 var maxSet := getMaxLengthSet(splitSets);
                 assert r.prepareQC.Cert? ==> ValidQC(r.prepareQC);
                 if |maxSet| >= quorum(|M_SpecTypes.All_Nodes|) && |maxSet| > 0
                 then
-                    assert forall m1, m2 | m1 in maxSet && m2 in maxSet :: m1.block == m2.block;
-                    assert forall m1, m2 | m1 in maxSet && m2 in maxSet :: m1.mType == m2.mType;
-                    assert forall m1, m2 | m1 in maxSet && m2 in maxSet :: m1.partialSig.signer != m2.partialSig.signer;
-                    assert forall m | m in maxSet :: m.mType == MT_Prepare;
+                    // assert forall m1, m2 | m1 in maxSet && m2 in maxSet :: m1.block == m2.block;
+                    // assert forall m1, m2 | m1 in maxSet && m2 in maxSet :: m1.mType == m2.mType;
+                    // assert forall m1, m2 | m1 in maxSet && m2 in maxSet && m1 != m2 :: m1.partialSig.signer != m2.partialSig.signer;
+                    // assert forall m | m in maxSet :: m.mType == MT_Prepare;
                     // assert forall m | m in maxSet :: m.block.Block?;
                     var m :| m in maxSet;
                     var sgns := ExtractSignatrues(maxSet);
                     var prepareQC := Cert(MT_Prepare, m.viewNum, m.block, sgns);
                     // assert ValidQC(prepareQC);
-                    // assert (&& prepareQC.Cert?
-                    //         && prepareQC.block.Block?
-                    //         && (forall s | s in prepareQC.signatures
-                    //                     ::  && s.Signature?
-                    //                         && s.mType == prepareQC.cType
-                    //                         && s.viewNum == prepareQC.viewNum
-                    //                         && s.block == prepareQC.block
-                    //                         && s.signer in All_Nodes
-                    //             )
-                    //         && (forall s1, s2 | && s1 in prepareQC.signatures 
-                    //                             && s2 in prepareQC.signatures
-                    //                             && s1 != s2
-                    //                         :: s1.signer != s2.signer
-                    //                         )
-                    //         && |prepareQC.signatures| >= quorum(|All_Nodes|));
                     var precommitMsg := Msg(MT_PreCommit, r.viewNum, EmptyBlock, prepareQC, SigNone);
-                    assert ValidQC(r'.prepareQC);
                     && outMsg == {precommitMsg}
-                    && r' == r.(msgReceived := r.msgReceived + {precommitMsg},
-                                msgSent := r.msgSent + {precommitMsg})
+                    && r' == r.(msgSent := r.msgSent + {precommitMsg})
                 else
                     assert r.prepareQC.Cert? ==> ValidQC(r.prepareQC);
                     && r' == r
@@ -601,10 +641,7 @@ module M_Replica {
             if |matchQCs| > 0 
             then 
                 var m :| m in matchQCs;
-                // var sig := Signature(r.id, m.cType, m.viewNum, m.block);
-                // var vote2 := Msg(MT_PreCommit, r.viewNum, m.block, CertNone, sig);
                 var vote := buildVoteMsg(MT_PreCommit, m.block, CertNone, r.viewNum, r.id);
-                // assert vote == vote2;
                 && outMsg == {vote}
                 && r' == r.(prepareQC := m,
                             msgSent := r.msgSent + {vote})
@@ -646,25 +683,23 @@ module M_Replica {
                     var commitMsg := Msg(MT_Commit, r.viewNum, EmptyBlock, precommitQC, SigNone);
                     assert ValidQC(m_qc);
                     && outMsg == {vote, commitMsg}
-                    && r' == r.(msgReceived := r.msgReceived + {commitMsg},
-                                msgSent := r.msgSent + {vote, commitMsg},
-                                commitQC := m_qc)
+                    && r' == r.(commitQC := m_qc,
+                                msgSent := r.msgSent + {vote, commitMsg})
                 else
                     assert ValidQC(m_qc);
                     && outMsg == {vote}
                     && r' == r.(commitQC := m_qc,
                                 msgSent := r.msgSent + {vote})
             else    // Only doing leader's work
-                var matchMsgs := getMatchMsg(r.msgReceived, MT_PreCommit, r.viewNum);
+                var matchMsgs := getMatchVoteMsg(r.msgReceived, MT_PreCommit, r.viewNum);
                 var splitSets := splitMsgByBlocks(matchMsgs);
                 var maxSet := getMaxLengthSet(splitSets);
                 // assert r.prepareQC.Cert? ==> ValidQC(r.prepareQC);
                 if |maxSet| >= quorum(|M_SpecTypes.All_Nodes|) && |maxSet| > 0
                 then
-                    assert false;
                     assert forall m1, m2 | m1 in maxSet && m2 in maxSet :: m1.block == m2.block;
                     assert forall m1, m2 | m1 in maxSet && m2 in maxSet :: m1.mType == m2.mType;
-                    assert forall m1, m2 | m1 in maxSet && m2 in maxSet :: m1.partialSig.signer != m2.partialSig.signer;
+                    assert forall m1, m2 | m1 in maxSet && m2 in maxSet :: m1.partialSig != m2.partialSig ==> m1.partialSig.signer != m2.partialSig.signer;
                     assert forall m | m in maxSet :: m.mType == MT_PreCommit;
                     // assert forall m | m in maxSet :: m.block.Block?;
                     var m :| m in maxSet;
@@ -689,8 +724,7 @@ module M_Replica {
                     var commitMsg := Msg(MT_Commit, r.viewNum, EmptyBlock, precommitQC, SigNone);
                     // assert ValidQC(r'.prepareQC);
                     && outMsg == {commitMsg}
-                    && r' == r.(msgReceived := r.msgReceived + {commitMsg},
-                                msgSent := r.msgSent + {commitMsg})
+                    && r' == r.(msgSent := r.msgSent + {commitMsg})
                 else
                     // assert r.prepareQC.Cert? ==> ValidQC(r.prepareQC);
                     && r' == r
@@ -715,70 +749,6 @@ module M_Replica {
                 && r' == r
     }
 
-    // ghost predicate UponCommit(r : ReplicaState, r' : ReplicaState, outMsg : set<Msg>)
-    // requires ValidReplicaState(r)
-    // {
-    //     var leader := leader(r.viewNum);
-    //     var matchMsgs := getMatchMsg(r.msgReceived, MT_PreCommit, r.viewNum);
-    //     var splitSets := splitMsgByBlocks(matchMsgs);
-    //     var maxSet := getMaxLengthSet(splitSets);
-
-    //     var matchQCs := getMatchQC(r.msgReceived, MT_PreCommit, r.viewNum);
-    //     // assert |matchQCs| > 0 && |matchMsgs| <= 0;
-    //     // assert |matchQCs| > 0 && |maxSet| >= quorum(|M_SpecTypes.All_Nodes|);
-    //     // assert |matchQCs| <= 0;
-    //     if leader == r.id // Leader
-    //     then
-    //         if |maxSet| >= quorum(|M_SpecTypes.All_Nodes|)
-    //         then
-    //             Axiom_Common_Constraints();
-    //             var m :| m in maxSet;
-    //             var sgns := ExtractSignatrues(maxSet);
-    //             var precommitQC := Cert(MT_PreCommit, m.viewNum, m.block, sgns);
-    //             var commitMsg := Msg(MT_Commit, r.viewNum, EmptyBlock, precommitQC, SigNone);
-    //             assert |matchQCs| <= 0;
-    //             if |matchQCs| > 0
-    //             then
-    //                 assert false;
-    //                 var m_qc :| m_qc in matchQCs;
-    //                 var sig := Signature(r.id, m_qc.cType, m_qc.viewNum, m_qc.block);
-    //                 var vote2 := Msg(MT_Commit, r.viewNum, m_qc.block, CertNone, sig);
-    //                 var vote := buildVoteMsg(MT_Commit, m.block, CertNone, r.viewNum, r.id);
-    //                 assert sig.mType == MT_PreCommit;
-    //                 assert vote.partialSig.mType == MT_Commit;
-    //                 && outMsg == {vote, commitMsg}
-    //                 && r' == r.(msgReceived := r.msgReceived + {commitMsg},
-    //                             msgSent := r.msgSent + outMsg,
-    //                             commitQC := precommitQC)
-    //             else
-    //                 && outMsg == {commitMsg}
-    //                 && r' == r.(msgReceived := r.msgReceived + {commitMsg},
-    //                             msgSent := r.msgSent + outMsg)
-    //         else
-    //             if |matchQCs| > 0
-    //             then
-    //                 var m_qc :| m_qc in matchQCs;
-    //                 var sig := Signature(r.id, m_qc.cType, m_qc.viewNum, m_qc.block);
-    //                 var vote := Msg(MT_Commit, r.viewNum, m_qc.block, CertNone, sig);
-    //                 && outMsg == {vote}
-    //                 && r' == r.(msgSent := r.msgSent + {vote})
-    //             else
-    //                 && outMsg == {}
-    //                 && r' == r
-    //     else    // Not a leader
-    //         if |matchQCs| > 0
-    //         then
-    //             var m_qc :| m_qc in matchQCs;
-    //             var sig := Signature(r.id, m_qc.cType, m_qc.viewNum, m_qc.block);
-    //             var vote := Msg(MT_Commit, r.viewNum, m_qc.block, CertNone, sig);
-    //             && outMsg == {vote}
-    //             && r' == r.(commitQC := m_qc,
-    //                         msgSent := r.msgSent + {vote})
-    //         else 
-    //             && outMsg == {}
-    //             && r' == r
-    // }
-
     ghost predicate UponDecide(r : ReplicaState, r' : ReplicaState, outMsg : set<Msg>)
     requires ValidReplicaState(r)
     {
@@ -802,8 +772,7 @@ module M_Replica {
                     var commitQC := Cert(MT_Commit, m.viewNum, m.block, sgns);
                     var decideMsg := Msg(MT_Decide, r.viewNum, EmptyBlock, commitQC, SigNone);
                     && outMsg == {decideMsg}
-                    && r' == r.(msgReceived := r.msgReceived + {decideMsg},
-                                msgSent := r.msgSent + {decideMsg})
+                    && r' == r.(msgSent := r.msgSent + {decideMsg})
                     && var ancestors := getAncestors(m_qc.block);
                     && (
                         || (
@@ -836,8 +805,7 @@ module M_Replica {
                     var sgns := ExtractSignatrues(maxSet);
                     var commitQC := Cert(MT_Commit, m.viewNum, m.block, sgns);
                     var decideMsg := Msg(MT_Decide, r.viewNum, EmptyBlock, commitQC, SigNone);
-                    && r' == r.(msgReceived := r.msgReceived + {decideMsg},
-                                msgSent := r.msgSent + {decideMsg})
+                    && r' == r.(msgSent := r.msgSent + {decideMsg})
                     && outMsg == {decideMsg}
                 else
                     && r' == r
@@ -878,58 +846,67 @@ module M_Replica {
         
     } 
 
-    ghost predicate ValidReplicaState(s : ReplicaState)
+    ghost predicate ValidReplicaState(r : ReplicaState)
     // requires M_SpecTypes.All_Nodes != {}
     {
         // TODO: invarians about a replica state
         //
         // && Inv_Node_Constraint()
-        && s.viewNum > 0
-        // The local blockchain should alwarys be consistent
-        // && Inv_Blockchain_Inner_Consistency(s.bc)
-        // If a replica accepted a commit certificate, 
-        // then the corresponding certified block should extend their local blockchain
-        // && (||(&& s.commitQC.Cert?
-        //        && s.commitQC.block.Block?
-        //        && s.bc <= getAncestors(s.commitQC.block)
-        //        )
-        //     ||(s.commitQC.CertNone?)
-        //     )
+        // && r.id in M_SpecTypes.All_Nodes
+        && r.viewNum > 0
         // If a replica accepted a Prepare certificate,
         // then it must received a PreCommit Message from the leader before, together with a valid Prepare certificate
-        && (s.prepareQC.Cert? ==>
-                                && ValidQC(s.prepareQC)
-                                && s.prepareQC.cType == MT_Prepare
-                                && exists m | m in s.msgReceived
+        && (r.prepareQC.Cert? ==>
+                                && ValidQC(r.prepareQC)
+                                && r.prepareQC.cType == MT_Prepare
+                                && exists m | m in r.msgReceived
                                             ::
                                             // && m.mType.MT_PreCommit?
-                                            && m.justify == s.prepareQC
+                                            && m.justify == r.prepareQC
             )
         // If a replica accepted a Precommit certificate (set it to its local variable `commitQC`),
         // then it must received a Commit Message from the leader before, together with a valid Precommit certificate
-        && (s.commitQC.Cert? ==>
-                                && ValidQC(s.commitQC)
-                                && s.commitQC.cType == MT_PreCommit
-                                && exists m | m in s.msgReceived
+        && (r.commitQC.Cert? ==>
+                                && ValidQC(r.commitQC)
+                                && r.commitQC.cType == MT_PreCommit
+                                && exists m | m in r.msgReceived
                                             ::
                                             // && m.mType.MT_Commit?
-                                            && m.justify == s.commitQC
+                                            && m.justify == r.commitQC
             )
         // If a replica received a Decide Message with a valid certificate,
         // then it should always update its local blockchain accordingly.
-        && (|| s.bc == [M_SpecTypes.Genesis_Block]
-            || (exists m | && m in s.msgReceived
+        && (|| r.bc == [M_SpecTypes.Genesis_Block]
+            || (exists m | && m in r.msgReceived
                         //    && m.mType.MT_Decide?
                            && m.justify.Cert?
                            && m.justify.cType.MT_Commit?
                            && ValidQC(m.justify)
                         //    && m.justify.block.Block?
                         ::
-                           s.bc <= getAncestors(m.justify.block)
+                           r.bc <= getAncestors(m.justify.block)
             )
         )
-        && |s.bc| > 0
-        && s.bc[0] == M_SpecTypes.Genesis_Block
+        && |r.bc| > 0
+        && r.bc[0] == M_SpecTypes.Genesis_Block
+        // && InvReplicaVote(s)
+        && (forall m | m in r.msgSent :: ValidMsg(m))
+    }
+
+    ghost predicate InvReplicaVote(r : ReplicaState)
+    {
+        forall m | && m in r.msgSent
+                   && ValidMsg(m)
+                :: 
+                   && m.partialSig.Signature?
+                   && m.partialSig.mType.MT_Commit?
+                   ==> 
+                   exists m2 | m2 in r.msgReceived
+                            ::
+                               && ValidMsg(m2)
+                               && ValidQC(m2.justify)
+                               && m2.justify.cType.MT_PreCommit?
+                               && m2.justify.block == m.partialSig.block
     }
 
     /**
@@ -947,9 +924,14 @@ module M_Replica {
                         && b[i1] == b[i2].parent
     }
 
-    opaque function getMsgReceive(r : ReplicaState) : (m : set<Msg>)
+    function getMsgReceiveReplica(r : ReplicaState) : (m : set<Msg>)
     {
         r.msgReceived
+    }
+
+    function getMsgSentReplica(r : ReplicaState) : (m : set<Msg>)
+    {
+        r.msgSent
     }
 
 }
